\documentclass[11pt, oneside]{article}   	% use "amsart" instead of "article" for AMSLaTeX format
\usepackage{geometry}                		% See geometry.pdf to learn the layout options. There are lots.
\usepackage{amsmath}
\geometry{letterpaper}                   		% ... or a4paper or a5paper or ... 
%\geometry{landscape}                		% Activate for rotated page geometry
%\usepackage[parfill]{parskip}    		% Activate to begin paragraphs with an empty line rather than an indent
\usepackage{graphicx}				% Use pdf, png, jpg, or epsÂ§ with pdflatex; use eps in DVI mode
								% TeX will automatically convert eps --> pdf in pdflatex		
\usepackage{amssymb}

%SetFonts

%SetFonts


\title{Brief Article}
\author{The Author}
%\date{}							% Activate to display a given date or no date

\begin{document}
\maketitle
%\section{}
%\subsection{}

$$\hat{H}=\hbar \omega_c  \hat{a}^{\dagger} \hat{a} + \frac{1}{2}\hbar \omega_a \hat{\sigma}_z+\frac{\hbar \Omega}{2}  \left(  \hat{a} +    \hat{a}^{\dagger}     \right) \left(  \hat{\sigma} +   \hat{\sigma}_-     \right)$$

$$\hat{H}= \omega_c  \hat{a}^{\dagger} \hat{a} + \omega_a \hat{\sigma}_z+g  \left(  \hat{a} +    \hat{a}^{\dagger}     \right) \left(  \hat{\sigma} +   \hat{\sigma}_-     \right)$$ %Original

$$\hat{H}= \omega_c  \hat{a}^{\dagger} \hat{a} + \omega_a \hat{\sigma}_z+g  \left(  \hat{a} +    \hat{a}^{\dagger}     \right) \left(  \hat{\sigma} +   \hat{\sigma}_-     \right)$$

$$ $$











$$\Delta v = c \Delta t \left(    v - \frac{v^3}{3} + w + I   \right) $$

$$\Delta w = -\frac{\Delta t}{c \tau} (v - a + bw ) $$

$\frac{dv}{dt}=c \left(  v - \frac{v^3}{3} + w + I \right) =0$
$ \implies w_1=-(v-\frac{v^3}{3}+I)=\frac{v^3}{3}-v-I$ \\
$\tau \frac{dw}{dt}=-\frac{1}{c}(v-a+bw)$
$\implies w_2 = \frac{1}{b}(a-v)$\\

$$\frac{dv}{dt}=c \left(  v - \frac{v^3}{3} + w + I \right) =0 \implies w_1=-(v-\frac{v^3}{3}+I)=\frac{v^3}{3}-v-I $$


$$\frac{dv}{dt}=c \left(  v - \frac{v^3}{3} - w + I \right) $$ 

$$ \frac{dw}{dt}=-\frac{1}{\tau c}(v+a-bw)$$


$$\frac{dv}{dt}=c (  v - \frac{v^3}{3} + w + I ) + k_1 \xi$$ 

$$ \frac{dw}{dt}=-\frac{1}{\tau c}(v-a+bw) + k_2 \eta$$


$$V_{i+1}=V_i + c \Delta t \left(       V_i -\frac{V_i^3}{3} +W_i +I  \right) $$

$$W_{i+1} = W_i - \frac{\Delta t}{c \tau} \left(  V_i - a + b W_i        \right) $$


$$V_{i+1}=V_i + c \Delta t \left(       V_i -\frac{V_i^3}{3} +W_i +I  \right) $$

$$W_{i+1} = W_i - \frac{\Delta t}{c \tau} \left(  V_i - a + b W_i        \right) $$


$$V_{i+1}=V_i + \Delta t \left(    c(   V_i -\frac{V_i^3}{3} +W_i +I ) + k_1 \xi  \right) $$

$$W_{i+1} = W_i + \Delta t  \left(  -\frac{1}{\tau c}(V_i - a + b W_i) +  k_2 \eta       \right) $$


$$\frac{\partial F(x,y)}{\partial X} =\left(
\begin{matrix}
\frac{\partial F_1 (x,y)}{\partial x} \\
\frac{\partial F_2 (x,y)}{\partial y}
\end{matrix} \right) $$

$$J=\left(
\begin{matrix}
\frac{\partial F_1(x,y)}{\partial x} & \frac{\partial F_1(x,y)}{\partial y} \\
\frac{\partial F_2(x,y)}{\partial x} & \frac{\partial F_2(x,y)}{\partial y}
\end{matrix}
\right) $$3



$$J=\left(
\begin{matrix}
c(1-v^2) & c \\
-\frac{1}{\tau c} & -\frac{b}{\tau c}
\end{matrix}
\right) $$

$$ dX_t = a(t,X_t) + b(t,X_t) dW_t$$

$$ X_{n+1} = X_n + a(t_n,X_n) \Delta t + b(t_n,X_n) \Delta W_n$$

$$ \Delta W_n = W_{t_{n+1}}-W_{t_{n}}$$

$$V_{i+1}=V_i + c\Delta t \left(       V_i -\frac{V_i^3}{3} +W_i +I   \right) +k_1 \sqrt{\Delta t} \xi $$

$$W_{i+1} = W_i - \frac{\Delta t}{c \tau} \left(  V_i - a + b W_i        \right)  + k_2 \sqrt{\Delta t} \eta $$


$$I = C_m \frac{dV_m}{dt} + \bar{g}_Kn^4 (V_m-V_k) + \bar{g}_{Na}m^3h(V_m-V_{Na}) + \bar{g}_l(V_m-V_l)$$
    
    $$\frac{dn}{dt} = \alpha_n (V_m)(1-n) - \beta_n (V_m) n$$

$$ \frac{dm}{dt} = \alpha_m (V_m)(1-m) - \beta_m (V_m) m$$

$$\frac{dh}{dt} = \alpha_h (V_m)(1-h) - \beta_h (V_m) h $$


















\end{document}  